src/Utils2.fsti
@@ -22,7 +22,7 @@ unfold let slab_metadata = r:array U64.t{A.length r = 4}
 
 //TODO: should not be hardcoded
 let page_size = 4096ul
-let metadata_max = 131072ul
+let metadata_max = 1048575ul
 
 noextract
 let min_sc = 64
